coq_new/sta_sr.v
@@ -49,8 +49,7 @@ Proof with eauto using sta0_type, sta0_wf, sta_step.
       apply: conv1i...
       exact: tyA'.
       exact: tym.
-      apply: sta0_pi0...
-      apply: sta_sta0_type... }
+      apply: sta0_pi0... }
     { have tym':=ihm _ H3.
       apply: sta0_lam0... } }
   { move=>Γ A B m s r tyA ihA tym ihm n st. inv st.
@@ -66,8 +65,7 @@ Proof with eauto using sta0_type, sta0_wf, sta_step.
       apply: conv1i...
       exact: tyA'.
       exact: tym.
-      apply: sta0_pi1...
-      apply: sta_sta0_type... }
+      apply: sta0_pi1... }
     { have tym':=ihm _ H3.
       apply: sta0_lam1... } }
   { move=>Γ A B m n s tym ihm tyn ihn x st. inv st.
@@ -108,6 +106,226 @@ Proof with eauto using sta0_type, sta0_wf, sta_step.
       move/sta0_sta_type in tyn.
       apply: sta_sta0_type.
       apply: sta_esubst... } }
+  { move=>Γ A B s r t ord tyA ihA tyB ihB n st. inv st.
+    { have tyA':=ihA _ H3.
+      move/sta0_sta_type in tyB.
+      move/sta0_sta_type in tyA'.
+      apply: sta0_sig0...
+      apply: sta_sta0_type.
+      apply: sta_ctx_conv.
+      apply: conv1i...
+      apply: tyA'.
+      apply: tyB. }
+    { have tyB':=ihB _ H3.
+      apply: sta0_sig0... } }
+  { move=>Γ A B s r t ord1 ord2 tyA ihA tyB ihB n st. inv st.
+    { have tyA':=ihA _ H3.
+      move/sta0_sta_type in tyB.
+      move/sta0_sta_type in tyA'.
+      apply: sta0_sig1.
+      apply: ord1. apply: ord2.
+      eauto.
+      apply: sta_sta0_type.
+      apply: sta_ctx_conv.
+      apply: conv1i...
+      apply: tyA'.
+      apply: tyB. }
+    { have tyB':=ihB _ H3.
+      apply: sta0_sig1.
+      apply: ord1. apply: ord2.
+      all: eauto. } }
+  { move=>Γ A B m n t tyS ihS tym ihm tyn ihn x st. inv st.
+    { have/sta0_sta_type tym':=ihm _ H3.
+      have tyS':=sta0_sta_type tyS.
+      have[r[tyB _]]:=sta_sig0_inv tyS'.
+      apply: sta0_pair0...
+      apply: sta0_conv.
+      apply: sta_conv_beta.
+      apply: conv1...
+      apply: tyn.
+      apply: sta_sta0_type.
+      apply: sta_esubst...
+      by autosubst. }
+    { have tyn':=ihn _ H3.
+      apply: sta0_pair0... } }
+  { move=>Γ A B m n t tyS ihS tym ihm tyn ihn x st. inv st.
+    { have/sta0_sta_type tym':=ihm _ H3.
+      have tyS':=sta0_sta_type tyS.
+      have[r[tyB _]]:=sta_sig1_inv tyS'.
+      apply: sta0_pair1...
+      apply: sta0_conv.
+      apply: sta_conv_beta.
+      apply: conv1...
+      apply: tyn.
+      apply: sta_sta0_type.
+      apply: sta_esubst...
+      by autosubst. }
+    { have tyn':=ihn _ H3.
+      apply: sta0_pair1... } }
+  { move=>Γ A B C m n s t tyC ihC tym ihm tyn ihn x st. inv st.
+    { have/sta0_sta_type tyA':=ihC _ H3.
+      move/sta0_sta_type in tyC.
+      move/sta0_sta_type in tym.
+      have//=tyCm:=sta_subst tyC tym.
+      have wf:=sta_type_wf tyC. inv wf.
+      have[r[tyB/sort_inj e]]:=sta_sig0_inv H2; subst.
+      have wf:=sta_type_wf tyB. inv wf.
+      have wkA':((Sig0 A B t).[ren (+2)] :: B :: A :: Γ) ⊢ A'.[ren (upren (+2))] : Sort s.
+      { replace (Sort s) with (Sort s).[ren (upren (+2))] by eauto.
+        apply: sta_rename...
+        apply: sta_agree_ren_cons...
+        replace (+2) with (id >>> (+1) >>> (+1)) by autosubst.
+        apply: sta_agree_ren_wk...
+        apply: sta_agree_ren_wk...
+        apply: sta_agree_ren_refl... }
+      have tyP:(B :: A :: Γ) ⊢ Pair0 (Var 1) (Var 0) t : (Sig0 A B t).[ren (+2)].
+      { apply: sta_pair0.
+        { replace (Sig0 A.[ren (+2)] B.[up (ren (+2))] t)
+          with (Sig0 A B t).[ren (+1)].[ren (+1)] by autosubst.
+          apply: sta_eweaken...
+          instantiate (1 := Sort t)=>//.
+          apply: sta_eweaken... eauto. }
+        { replace A.[ren (+2)] with A.[ren (+1)].[ren (+1)] by autosubst.
+          repeat constructor.
+          econstructor... }
+        { asimpl.
+          repeat constructor.
+          econstructor... } }
+      have{}xA':=sta_subst wkA' tyP. asimpl in xA'.
+      apply:sta0_conv.
+      apply: sta_conv_subst.
+      apply: conv1i...
+      apply: sta0_letin0...
+      apply: sta0_conv.
+      apply: sta_conv_subst.
+      apply: conv1...
+      apply: tyn.
+      apply: sta_sta0_type...
+      eauto. }
+    { have/sta0_sta_type tym':=ihm _ H3.
+      move/sta0_sta_type in tyC.
+      move/sta0_sta_type in tym.
+      have//=tyCm:=sta_subst tyC tym.
+      apply: sta0_conv.
+      apply: sta_conv_beta.
+      apply: conv1i...
+      apply: sta0_letin0...
+      eauto... }
+    { have tyn':=ihn _ H3. apply: sta0_letin0... }
+    { move/sta0_sta_type in tyn.
+      move/sta0_sta_type in tym.
+      have[e[tym1 tym2]]:=sta_pair0_inv tym; subst.
+      apply: sta_sta0_type.
+      replace C.[Pair0 m1 m2 t/]
+        with C.[Pair0 (Var 1) (Var 0) t .: ren (+2)].[m2,m1/] by autosubst.
+      apply: sta_substitution...
+      repeat constructor...
+      by asimpl. }
+    { move/sta0_sta_type in tym.
+      exfalso. apply: sta_pair1_sig0_false... } }
+  { move=>Γ A B C m n s t tyC ihC tym ihm tyn ihn x st. inv st.
+    { have/sta0_sta_type tyA':=ihC _ H3.
+      move/sta0_sta_type in tyC.
+      move/sta0_sta_type in tym.
+      have//=tyCm:=sta_subst tyC tym.
+      have wf:=sta_type_wf tyC. inv wf.
+      have[r[tyB/sort_inj e]]:=sta_sig1_inv H2; subst.
+      have wf:=sta_type_wf tyB. inv wf.
+      have wkA':((Sig1 A B t).[ren (+2)] :: B :: A :: Γ) ⊢ A'.[ren (upren (+2))] : Sort s.
+      { replace (Sort s) with (Sort s).[ren (upren (+2))] by eauto.
+        apply: sta_rename...
+        apply: sta_agree_ren_cons...
+        replace (+2) with (id >>> (+1) >>> (+1)) by autosubst.
+        apply: sta_agree_ren_wk...
+        apply: sta_agree_ren_wk...
+        apply: sta_agree_ren_refl... }
+      have tyP:(B :: A :: Γ) ⊢ Pair1 (Var 1) (Var 0) t : (Sig1 A B t).[ren (+2)].
+      { apply: sta_pair1.
+        { replace (Sig1 A.[ren (+2)] B.[up (ren (+2))] t)
+          with (Sig1 A B t).[ren (+1)].[ren (+1)] by autosubst.
+          apply: sta_eweaken...
+          instantiate (1 := Sort t)=>//.
+          apply: sta_eweaken... eauto. }
+        { replace A.[ren (+2)] with A.[ren (+1)].[ren (+1)] by autosubst.
+          repeat constructor.
+          econstructor... }
+        { asimpl.
+          repeat constructor.
+          econstructor... } }
+      have{}xA':=sta_subst wkA' tyP. asimpl in xA'.
+      apply:sta0_conv.
+      apply: sta_conv_subst.
+      apply: conv1i...
+      apply: sta0_letin1...
+      apply: sta0_conv.
+      apply: sta_conv_subst.
+      apply: conv1...
+      apply: tyn.
+      apply: sta_sta0_type...
+      eauto. }
+    { have/sta0_sta_type tym':=ihm _ H3.
+      move/sta0_sta_type in tyC.
+      move/sta0_sta_type in tym.
+      have//=tyCm:=sta_subst tyC tym.
+      apply: sta0_conv.
+      apply: sta_conv_beta.
+      apply: conv1i...
+      apply: sta0_letin1...
+      eauto... }
+    { have tyn':=ihn _ H3. apply: sta0_letin1... }
+    { move/sta0_sta_type in tym.
+      exfalso. apply: sta_pair0_sig1_false... }
+    { move/sta0_sta_type in tyn.
+      move/sta0_sta_type in tym.
+      have[e[tym1 tym2]]:=sta_pair1_inv tym; subst.
+      apply: sta_sta0_type.
+      replace C.[Pair1 m1 m2 t/]
+        with C.[Pair1 (Var 1) (Var 0) t .: ren (+2)].[m2,m1/] by autosubst.
+      apply: sta_substitution...
+      repeat constructor...
+      by asimpl. } }
+  { move=>Γ A B s r t tyA ihA tyB ihB n st. inv st.
+    { have tyA':=ihA _ H3. apply: sta0_with... }
+    { have tyB':=ihB _ H3. apply: sta0_with... } }
+  { move=>Γ A B m n t tym ihm tyn ihn n0 st. inv st.
+    { have tym':=ihm _ H3. apply: sta0_apair... }
+    { have tyn':=ihn _ H3. apply: sta0_apair... } }
+  { move=>Γ A B m t tym ihm n st. inv st.
+    { have tym':=ihm _ H0. apply: sta0_fst... }
+    { move/sta0_sta_type in tym.
+      have[_[tyn _]]:=sta_apair_inv tym... } }
+  { move=>Γ A B m t tym ihm n st. inv st.
+    { have tym':=ihm _ H0. apply: sta0_snd... }
+    { move/sta0_sta_type in tym.
+      have[_[_ tyn]]:=sta_apair_inv tym... } }
+  { move=>Γ A m n s tyA ihA tym ihm tyn ihn n0 st. inv st.
+    { have tyA':=ihA _ H3.
+      apply: sta0_id...
+      apply: sta0_conv.
+      apply: conv1...
+      all: eauto.
+      apply: sta0_conv.
+      apply: conv1...
+      all: eauto. }
+    { have tym':=ihm _ H3. apply: sta0_id... }
+    { have tyn':=ihn _ H3. apply: sta0_id... } }
+  { move=>Γ A m tym ihm n st. inv st.
+    move/sta0_sta_type in tym.
+    have[s tyA]:=sta_valid tym.
+    have tym':=ihm _ H0.
+    apply: sta0_conv.
+    apply: sta_conv_id.
+    eauto.
+    apply: conv1i...
+    apply: conv1i...
+    apply: sta0_refl...
+    apply: sta0_id... }
+  { move=>Γ A B H P m n s tyB ihB tyH ihH tyP ihP n0 st. inv st.
+    {
+
+    }
+
+  }
 Qed.
 
 Corollary sta_rd Γ m n A :
